Freigen.lean
@@ -1,8 +1,8 @@
 -- This module serves as the root of the `Freigen` library.
 import Freigen.Free
 import Freigen.Ast
-import Freigen.Reflect
-import Freigen.Domain
 import Freigen.ITree
-import Freigen.DenoteITree
+import Freigen.Eutt
+import Freigen.Adequacy
+import Freigen.Reflect
 import Freigen.Examples
